IMPminus_TM/Def/Global_Defs.thy
@@ -12,7 +12,10 @@ fun inth :: "'a list \<Rightarrow> nat \<Rightarrow> 'a" (infixl "!!" 100) where
   "[] !! i = undefined" |
   "(x # xs) !! i = (if i = 1 then x else xs !! (i - 1))"
 
-text \<open>The only additional lemma we need about this function is indexing over append:\<close>
+lemma inth_mem[intro]:
+  "0 < i \<Longrightarrow> i \<le> length xs \<Longrightarrow> xs !! i \<in> set xs"
+  by (induction xs arbitrary: i) auto
+
 lemma inth_append [simp]:
   "0 < i \<Longrightarrow> i \<le> length xs + length ys \<Longrightarrow> xs \<noteq> [] \<Longrightarrow> ys \<noteq> [] \<Longrightarrow>
   (xs @ ys) !! i = (if i \<le> size xs then xs !! i else ys !! (i - size xs))" 
@@ -20,5 +23,10 @@ lemma inth_append [simp]:
   apply (metis Suc_le_mono Suc_pred diff_is_0_eq list.size(3) neq0_conv trans_le_add1)
   by (smt (verit, ccfv_threshold) Suc_pred append_Nil diff_Suc_Suc diff_is_0_eq le0 list.size(3) neq0_conv)
 
+lemma inth_append_in_fst_list [simp]:
+  "0 < i \<Longrightarrow> i \<le> length xs \<Longrightarrow> xs \<noteq> [] \<Longrightarrow> (xs @ ys) !! i = xs !! i"
+  apply (induction xs arbitrary: i)
+  apply auto
+  by (metis Suc_le_mono Suc_pred diff_is_0_eq length_0_conv not_gr_zero)
 
 end
